lean/STLC/STLC/Smallstep_FullBeta_LR.lean
@@ -1,0 +1,397 @@
+-- STLC with full beta-reduction
+-- locally nameless where free variables are de Bruijn levels
+-- small-step semantics and unary logical relation
+-- following Kripke-Style Logical Relations for Normalization, Robert Harper
+
+import Mathlib.Data.Finset.Sort
+import STLC.Env
+
+namespace Smallstep_Equiv_Beta
+
+inductive ty : Type
+| bool : ty
+| arrow : ty → ty → ty
+
+inductive tm : Type
+| fls : tm
+| tru : tm
+| bvar : ℕ → tm
+| fvar : ℕ → tm
+| abs : tm → tm
+| app : tm → tm → tm
+
+abbrev tenv := List ty
+abbrev venv := List tm
+
+-- combine open and subst: t1[n ↦ t2]
+@[simp]
+def openSubst (t1: tm) (n: ℕ) (t2: tm) : tm :=
+  match t1 with
+  | .fls | .tru => t1
+  | .bvar x =>
+    if x = n then t2
+    else if n < x then .bvar (x - 1)
+    else .bvar x
+  | .fvar x => .fvar x
+  | .abs t1 => .abs (openSubst t1 (n + 1) t2)
+  | .app t11 t12 =>
+    .app (openSubst t11 n t2) (openSubst t12 n t2)
+
+@[simp]
+def substF (Δ: venv) (t: tm) : tm :=
+  match t with
+  | .fls | .tru => t
+  | .bvar _ => t
+  | .fvar x =>
+    match indexr x Δ with
+    | none => t
+    | some t' => t'
+  | .abs t1 => .abs (substF Δ t1)
+  | .app t11 t12 => .app (substF Δ t11) (substF Δ t12)
+
+@[simp]
+def closedF (t: tm) (n: ℕ) : Prop :=
+  match t with
+  | .fls | .tru => true
+  | .bvar _ => true
+  | .fvar x => x < n
+  | .abs t1 => closedF t1 n
+  | .app t11 t12 => closedF t11 n ∧ closedF t12 n
+
+@[simp]
+def closedB (t: tm) (n: ℕ) : Prop :=
+  match t with
+  | .fls | .tru => true
+  | .bvar x => x < n
+  | .fvar _ => true
+  | .abs t1 => closedB t1 (n + 1)
+  | .app t11 t12 => closedB t11 n ∧ closedB t12 n
+
+lemma openClosed : ∀ t n m,
+  closedB (openSubst t m (.fvar n)) m →
+  closedB t (m+1) := by
+  intros t; induction t <;> intros n m h <;> simp
+  case bvar x =>
+    by_cases hx: (x = m)
+    . omega
+    . by_cases hx': (x < m)
+      omega; unfold openSubst at h;
+      rw [if_neg hx] at h; have hx'' : (m < x) := by omega;
+      simp [hx''] at h; omega
+  case abs t ih =>
+    apply ih n (m+1); simp at h; assumption
+  case app t1 t2 ih1 ih2 =>
+    apply And.intro; apply ih1 n m h.1; apply ih2 n m h.2
+
+lemma openClosed': ∀ t n m,
+    closedB t (m+1) → closedB (openSubst t m (.fvar n)) m := by
+  intros t; induction t <;> intros n m h <;> simp
+  case bvar x =>
+    by_cases hx: (x = m)
+    . simp [hx]
+    . rw [if_neg hx]; by_cases hx': (m < x)
+      . simp at h; omega
+      . rw [if_neg hx']; simp; omega
+  case abs t ih =>
+    apply ih n (m+1); simp at h; assumption
+  case app t1 t2 ih1 ih2 =>
+    apply And.intro; apply ih1 n m h.1; apply ih2 n m h.2
+
+lemma closedBOpenId: ∀ t1 t2 n,
+  closedB t1 n -> openSubst t1 n t2 = t1 := by
+  intros t1; induction t1 <;> intros t2 n h <;> simp
+  case bvar x =>
+    by_cases hx: (x = n)
+    . simp at h; omega
+    . rw [if_neg hx]; by_cases hx': (n < x)
+      . simp at h; omega
+      . simp [if_neg hx']
+  case abs t ih => simp at h; apply ih; assumption
+  case app t1 t2 ih1 ih2 =>
+    apply And.intro
+    . apply ih1; apply h.1
+    . apply ih2; apply h.2
+
+lemma closedBInc: ∀ t n n1,
+    closedB t n -> n <= n1 -> closedB t n1 := by
+  intros t; induction t <;> intros n n1 hcl hle <;> simp
+  case bvar x => simp at hcl; omega
+  case abs t ih => simp at hcl; apply ih; apply hcl; omega
+  case app t1 t2 ih1 ih2 =>
+    apply And.intro
+    . apply ih1; apply hcl.1; omega
+    . apply ih2; apply hcl.2; omega
+
+lemma closedFInc: ∀ t n k, closedF t n -> closedF (openSubst t k (tm.fvar n)) (n + 1) := by
+  intros t; induction t <;> intros n k hcl <;> simp
+  case fvar x => simp at hcl; omega
+  case bvar x =>
+    by_cases hx: (x = k)
+    . simp [hx];
+    . rw [if_neg hx];
+      by_cases hx': (k < x)
+      . simp [hx']
+      . rw [if_neg hx']; simp
+  case abs t ih => apply ih; simp at hcl; assumption
+  case app t1 t2 ih1 ih2 =>
+    apply And.intro
+    . apply ih1; apply hcl.1
+    . apply ih2; apply hcl.2
+
+lemma substFOpenComm : ∀ t t1 Δ n, closedF t Δ.length →
+  (∀ x t1, indexr x Δ = some t1 → closedB t1 0) →
+  substF (t1::Δ) (openSubst t n (.fvar Δ.length)) =
+  openSubst (substF Δ t) n t1 := by
+  intros t t1 Δ n h; revert n; induction t <;> intros n hc <;> simp
+  case bvar x =>
+    by_cases hx: (x = n)
+    . simp [hx]
+    . rw [if_neg hx]; rw [if_neg hx]
+      by_cases hx': (n < x)
+      simp [hx']; rw [if_neg hx']; simp
+  case fvar x =>
+    have h' := indexrSome Δ x h
+    rcases h' with ⟨v, hidx⟩; rw [hidx]; simp;
+    have hx : ¬(x = Δ.length) := by simp at h; omega
+    rw [if_neg hx]; simp;
+    rw [closedBOpenId]; apply closedBInc; apply hc; apply hidx; omega
+  case abs t ih => apply ih; simp at h; assumption; apply hc
+  case app t1 t2 ih1 ih2 =>
+    simp at h; apply And.intro
+    . apply ih1; apply h.1; assumption
+    . apply ih2; apply h.2; assumption
+
+lemma substFClosedBComm: ∀ t Δ n,
+  (forall x t1, indexr x Δ = some t1 -> closedB t1 0) ->
+  (closedB t n) -> (closedB (substF Δ t) n) := by
+  intros t; induction t <;> intros E n hidx hcl <;> simp
+  case bvar x => simp at hcl; assumption
+  case fvar x =>
+    generalize h : indexr x E = v
+    cases v <;> simp
+    case some v => apply closedBInc; apply hidx; apply h; omega
+  case abs t ih => apply ih; apply hidx; simp at hcl; assumption
+  case app t1 t2 ih1 ih2 =>
+    rcases hcl with ⟨hcl1, hcl2⟩
+    apply And.intro
+    . apply ih1; apply hidx; assumption
+    . apply ih2; apply hidx; assumption
+
+@[simp]
+def binds x τ (Γ : tenv) := (indexr x Γ = some τ)
+
+inductive hasType : tenv → tm → ty → Prop
+| fls : ∀ Γ, hasType Γ .fls .bool
+| tru : ∀ Γ, hasType Γ .tru .bool
+| var : ∀ Γ x τ, binds x τ Γ → hasType Γ (.fvar x) τ
+| abs : ∀ Γ t τ₁ τ₂,
+  hasType (τ₁::Γ) (openSubst t 0 (.fvar Γ.length)) τ₂ →
+  closedF t Γ.length →
+  hasType Γ (.abs t) (ty.arrow τ₁ τ₂)
+| app : ∀ Γ t₁ t₂ τ₁ τ₂,
+  hasType Γ t₁ (.arrow τ₁ τ₂) →
+  hasType Γ t₂ τ₁ →
+  hasType Γ (.app t₁ t₂) τ₂
+
+inductive value : tm → Prop
+| fls : value .fls
+| tru : value .tru
+| abs : ∀ t, value (.abs t)
+
+inductive step : tm → tm → Prop
+| beta : ∀ t1 t2,
+  step (.app (.abs t1) t2) (openSubst t1 0 t2)
+| app1 : ∀ t1 t1' t2,
+  step t1 t1' →
+  step (.app t1 t2) (.app t1' t2)
+| app2 : ∀ t1 t2 t2',
+  step t2 t2' →
+  step (.app t1 t2) (.app t1 t2')
+| lam : ∀ t1 t2,
+  step t1 t2 →
+  step (.abs t1) (.abs t2)
+
+inductive stepn : tm → tm → Prop
+| refl : ∀ t, stepn t t
+| multi : ∀ t1 t2 t3, stepn t1 t2 → step t2 t3 → stepn t1 t3
+
+lemma stepnApp1 : ∀ t1 t1' t2, stepn t1 t1' → stepn (.app t1 t2) (.app t1' t2) := by
+  intros t1 t1' t2 h; induction h
+  . constructor
+  . case _ hstn hst ih => constructor; assumption; apply step.app1; assumption
+
+lemma stepnApp2 : ∀ t1 t2 t2', stepn t2 t2' → stepn (.app t1 t2) (.app t1 t2') := by
+  intros t1 t2 t2' h; induction h
+  . constructor
+  . case _ hstn hst ih => apply stepn.multi; assumption; apply step.app2; assumption
+
+lemma stepnLam : ∀ t1 t2, stepn t1 t2 → stepn (.abs t1) (.abs t2) := by
+  intros t1 t2 h; induction h
+  . constructor
+  . case _ hstn hst ih => apply stepn.multi; assumption; apply step.lam; assumption
+
+lemma stepnTrans : ∀ t1 t2 t3, stepn t1 t2 → stepn t2 t3 → stepn t1 t3 := by
+  intros t1 t2 t3 h1 h2; induction h2
+  . assumption
+  . case _ _ _ hstn hst ih =>
+    apply stepn.multi; apply ih; assumption
+
+lemma stepn.multi' : ∀ t1 t2 t3, step t1 t2 → stepn t2 t3 → stepn t1 t3 := by
+  intros t1 t2 t3 st1 st2
+  have st3 : stepn t1 t1 := by constructor
+  have st4 : stepn t1 t2 := by apply stepn.multi; assumption; apply st1
+  apply stepnTrans; assumption; assumption
+
+def extend (Γ1 Γ2 : tenv) : Prop :=
+  ∀ x τ, hasType Γ1 (.fvar x) τ → hasType Γ2 (.fvar x) τ
+
+notation:60 a:65 "≤" b:65 => extend a b
+
+lemma extendRefl : ∀ Γ, Γ ≤ Γ := by intros Γ x τ hty; assumption
+
+lemma extend1 : ∀ τ Γ, Γ ≤ (τ :: Γ) := by
+  intros τ Γ x τ hty
+  rcases hty; case var τ1 hbd =>
+    by_cases hx: (x >= Γ.length);
+    . simp at hbd; rw [indexrNone] at hbd; cases hbd; omega
+    . constructor; simp; aesop
+
+lemma extendTrans : ∀ Γ1 Γ2 Γ3,
+  Γ1 ≤ Γ2 → Γ2 ≤ Γ3 → Γ1 ≤ Γ3 := by
+  intros Γ1 Γ2 Γ3 hE1 hE2 x τ hT;
+  apply hE2; apply hE1; assumption
+
+@[simp]
+def βnorm (t: tm) : Prop := ¬ ∃ t', step t t'
+
+@[simp]
+def normalizable (t: tm) : Prop := ∃ t', stepn t t' ∧ βnorm t'
+
+-- hereditary normalization
+@[simp]
+def HN (Γ: tenv) (t: tm) (τ: ty): Prop :=
+  match τ with
+  | .bool => normalizable t
+  | .arrow τ1 τ2 =>
+    ∀ Γ' t1, Γ ≤ Γ' → closedB t1 0 → HN Γ' t1 τ1 → HN Γ' (.app t t1) τ2
+
+lemma monotonicity : ∀ Γ1 Γ2 t τ, Γ2 ≤ Γ1 → HN Γ2 t τ → HN Γ1 t τ := by
+  intros Γ1 Γ2 t τ hE hv; induction τ
+  case bool => exact hv
+  case arrow τ1 τ2 ih1 ih2 =>
+    intros Γ' t1 hE' hvalt1
+    apply hv; apply extendTrans; apply hE; apply hE'; assumption
+
+lemma headExpansion : ∀ Γ t1 t2 τ, step t1 t2 → HN Γ t2 τ → HN Γ t1 τ := by
+  intros Γ t1 t2 τ hst hv
+  induction τ generalizing Γ t1 t2
+  case bool =>
+    simp at hv; simp; rcases hv with ⟨v, hstn, hnorm⟩
+    exists v; constructor; apply stepn.multi'; apply hst
+    apply hstn; apply hnorm
+  case arrow τ1 τ2 ih1 ih2 =>
+    intro Γ' t1' hE hvalt1'
+    have hst' : step (t1.app t1') (t2.app t1') := by constructor; assumption
+    aesop
+
+@[simp]
+def envType (Δ : tenv) (Γ : tenv) (γ : venv) : Prop :=
+  Γ.length = γ.length ∧
+  ∀ τ x, binds x τ Γ →
+  ∃ v, indexr x γ = some v ∧ closedB v 0 ∧ HN Δ v τ
+
+lemma monoEnv : ∀ Δ1 Δ2 Γ γ, Δ2 ≤ Δ1 →
+  envType Δ2 Γ γ → envType Δ1 Γ γ := by
+  intros Δ1 Δ2 Γ γ hE henv; rcases henv with ⟨hlen, h⟩
+  constructor; assumption; intros τ x hbd
+  specialize h τ x hbd
+  rcases h with ⟨v, hidx, hcl, hv⟩
+  exists v; constructor; assumption; constructor; assumption
+  apply monotonicity; assumption; assumption
+
+lemma envTypeMt : ∀ Δ, envType Δ [] [] := by simp
+
+lemma envTypeExtend : ∀ Δ Γ γ v τ,
+  envType Δ Γ γ → closedB v 0 → HN Δ v τ → envType Δ (τ::Γ) (v::γ) := by
+  intros Δ Γ γ v τ henv hcl hv; simp; simp at henv
+  apply And.intro
+  . apply henv.1
+  . intros τ1 x bd; rcases henv with ⟨hlen, h⟩
+    by_cases hx: (x = Γ.length)
+    . rw [hx] at bd; simp at bd
+      rw [hx, hlen]; simp [hx]; rw [<-bd]; apply And.intro <;> assumption
+    . rw [if_neg hx] at bd; rw [<-hlen]; rw [if_neg hx]
+      specialize h τ1 x bd; rcases h with ⟨v, hidx, hclv, hv⟩; exists v
+
+lemma envTypeClosed : ∀ Δ Γ γ, envType Δ Γ γ →
+  (∀ x t1, indexr x γ = some t1 → closedB t1 0) := by
+  intros Δ Γ γ henv; rcases henv with ⟨hlen, h⟩
+  intros x t1 hidx;
+  have hx : (x < γ.length) := by apply indexrSome'; exists t1
+  rw [<-hlen] at hx; have hidx' := indexrSome Γ x hx
+  rcases hidx' with ⟨τ, hidx'⟩;
+  have ⟨t2, hidx'', hval⟩  := h τ x hidx'
+  rcases hval with ⟨hcl, _⟩; rw [hidx] at hidx''; cases hidx''; assumption
+
+@[simp]
+def semType (Γ : tenv) (t : tm) (τ : ty) : Prop :=
+  ∀ Δ γ, closedB t 0 → envType Δ Γ γ → HN Δ (substF γ t) τ
+
+lemma semFls: ∀ Γ, semType Γ .fls .bool := by
+  intros Γ Δ γ hcl henv; simp; rcases henv with ⟨hlen, h⟩
+  exists .fls; constructor; apply stepn.refl; intros x f; cases f
+
+lemma semTru: ∀ Γ, semType Γ .tru .bool := by
+  intros Γ Δ γ hcl henv; simp; rcases henv with ⟨hlen, h⟩
+  exists .tru; constructor; apply stepn.refl; intros x f; cases f
+
+lemma semVar: ∀ Γ x τ, binds x τ Γ → semType Γ (.fvar x) τ := by
+  intros Γ x τ bd Δ γ hcl henv; simp
+  rcases henv with ⟨hlen, henv⟩
+  rcases henv _ _ bd with ⟨w, h⟩
+  simp [h.1]; exact h.2.2
+
+lemma semApp: ∀ Γ f t τ1 τ2,
+  semType Γ f (.arrow τ1 τ2) →
+  semType Γ t τ1 →
+  semType Γ (.app f t) τ2 := by
+  intros Γ f t τ1 τ2 hsemf hsemt Δ γ hcl henv
+  rcases hcl  with ⟨hclf, hclt⟩
+  specialize hsemf Δ γ hclf henv
+  specialize hsemt Δ γ hclt henv
+  have he : extend Δ Δ := by apply extendRefl
+  have hcl : closedB (substF γ t) 0 := by
+    apply substFClosedBComm; apply envTypeClosed Δ Γ γ henv; assumption
+  specialize hsemf Δ (substF γ t) he hcl hsemt
+  simp; assumption
+
+lemma semAbs: ∀ Γ t τ1 τ2,
+  semType (τ1::Γ) (openSubst t 0 (.fvar Γ.length)) τ2 →
+  closedF t Γ.length →
+  semType Γ (.abs t) (.arrow τ1 τ2) := by
+  intros Γ t τ1 τ2 hsemt hclosed Δ γ hcl henv
+  intros Γ' t1 he hclt1 hvalt1; simp; simp at hcl
+  have hcl' := openClosed' t (Γ.length) 0 hcl
+  have henv' : envType Γ' Γ γ := by apply monoEnv <;> assumption
+  have henv'' : envType Γ' (τ1::Γ) (t1::γ) := by apply envTypeExtend <;> assumption
+  specialize hsemt Γ' (t1::γ) hcl' henv''
+  rw [henv.1, substFOpenComm] at hsemt
+  have st : step ((substF γ t).abs.app t1) (openSubst (substF γ t) 0 t1) := by apply step.beta
+  apply headExpansion; assumption; assumption
+  rw [<-henv.1]; assumption
+  apply envTypeClosed Δ Γ γ henv
+
+lemma fundamental : ∀ Γ t τ,
+  hasType Γ t τ → semType Γ t τ := by
+  intros Γ t τ hty
+  induction hty
+  case fls => apply semFls
+  case tru => apply semTru
+  case var x τ hbd => apply semVar; assumption
+  case abs τ1 τ2 t ih hcl => apply semAbs; assumption; assumption
+  case app t1 t2 τ1 τ2 ih1 ih2 =>
+    apply semApp; assumption; assumption
+
+
+
+end Smallstep_Equiv_Beta
